Continued work on cleaning up assembly

12AssemblyCode/AssemblyCode.thy
@@ -4,103 +4,125 @@ begin
 
 datatype register = Hp | Env | Vals | Stk
 
-datatype pseudoreg = Reg register | PC nat | Con nat | PAcc pseudoreg
+datatype move_src = Reg "register option" | Con nat 
 
 datatype assm = 
-  AMov pseudoreg
-  | AGet "register option"
-  | APut register pseudoreg
+  AGet "register option"
+  | APut "register option" move_src
   | ASub "register option" nat
   | AAdd "register option" nat
   | AJmp
 
 datatype assm_state = 
-  AS "register \<Rightarrow> nat \<Rightarrow> register option \<times> nat" "register \<Rightarrow> nat" nat "register option" nat
+  AS "register option \<Rightarrow> nat \<Rightarrow> register option \<times> nat" "register option \<Rightarrow> nat" "register option" nat
 
-fun mem_upd :: "(register \<Rightarrow> nat \<Rightarrow> register option \<times> nat) \<Rightarrow> register \<Rightarrow> nat \<Rightarrow> 
-    register option \<times> nat \<Rightarrow> register \<Rightarrow> nat \<Rightarrow> register option \<times> nat" where
+primrec registers_case :: "'a \<Rightarrow> 'a \<Rightarrow> 'a \<Rightarrow> 'a \<Rightarrow> 'a \<Rightarrow> register option \<Rightarrow> 'a" where
+  "registers_case hp ep vp sp a (Some r) = case_register hp ep vp sp r"
+| "registers_case hp ep vp sp a None = a"
+
+fun mem_upd :: "(register option \<Rightarrow> nat \<Rightarrow> register option \<times> nat) \<Rightarrow> register option \<Rightarrow> nat \<Rightarrow> 
+    register option \<times> nat \<Rightarrow> register option \<Rightarrow> nat \<Rightarrow> register option \<times> nat" where
   "mem_upd mem m mp k m' x = (if m = m' \<and> mp = x then k else mem m' x)"
 
-fun assm_step :: "(register \<Rightarrow> nat \<Rightarrow> register option \<times> nat) \<Rightarrow> (register \<Rightarrow> nat) \<Rightarrow> nat \<Rightarrow> 
+fun assm_step :: "(register option \<Rightarrow> nat \<Rightarrow> register option \<times> nat) \<Rightarrow> (register option \<Rightarrow> nat) \<Rightarrow>
     register option \<Rightarrow> nat \<Rightarrow> assm \<rightharpoonup> assm_state" where
-  "assm_step mem ps a act pc (AMov (Reg r)) = Some (AS mem ps (ps r) (Some r) pc)"
-| "assm_step mem ps a act pc (AMov (PC _)) = Some (AS mem ps pc None pc)"
-| "assm_step mem ps a act pc (AMov (Con k)) = Some (AS mem ps k None pc)"
-| "assm_step mem ps a act pc (AMov (PAcc _)) = None"
-| "assm_step mem ps a act pc (AGet (Some r)) = (case mem r (ps r) of
-      (t, b) \<Rightarrow> Some (AS mem ps b t pc))"
-| "assm_step mem ps a None pc (AGet None) = None"
-| "assm_step mem ps a (Some r) pc (AGet None) = (case mem r a of
-      (t, b) \<Rightarrow> Some (AS mem ps b t pc))"
-| "assm_step mem ps a act pc (APut r (Reg r')) = 
-    Some (AS (mem_upd mem r (ps r) (Some r', ps r')) ps a act pc)"
-| "assm_step mem ps a act pc (APut r (PC k)) = 
-    Some (AS (mem_upd mem r (ps r) (None, k)) ps a act pc)"
-| "assm_step mem ps a act pc (APut r (Con k)) = 
-    Some (AS (mem_upd mem r (ps r) (None, k)) ps a act pc)"
-| "assm_step mem ps a act pc (APut r (PAcc t)) = 
-    Some (AS (mem_upd mem r (ps r) (act, a)) ps a act pc)" 
-| "assm_step mem ps a act pc (ASub (Some r) k) = 
-    (if ps r \<ge> k then Some (AS mem (ps(r := ps r - k)) a act pc) else None)"
-| "assm_step mem ps a None pc (ASub None k) = None"
-| "assm_step mem ps a (Some r) pc (ASub None k) =
-    (if a \<ge> k then Some (AS mem ps (a - k) (Some r) pc) else None)"
-| "assm_step mem ps a act pc (AAdd (Some r) k) = Some (AS mem (ps(r := ps r + k)) a act pc)"
-| "assm_step mem ps a None pc (AAdd None k) = None"
-| "assm_step mem ps a (Some r) pc (AAdd None k) = Some (AS mem ps (a + k) (Some r) pc)"
-| "assm_step mem ps a None pc AJmp = Some (AS mem ps 0 None a)"
-| "assm_step mem ps a (Some r) pc AJmp = None"
+  "assm_step mem ps act pc (AGet (Some r)) = (case mem (Some r) (ps (Some r)) of
+      (t, b) \<Rightarrow> Some (AS mem (ps(None := b)) t pc))"
+| "assm_step mem ps None pc (AGet None) = None"
+| "assm_step mem ps (Some r) pc (AGet None) = (case mem (Some r) (ps None) of
+      (t, b) \<Rightarrow> Some (AS mem (ps(None := b)) t pc))"
+| "assm_step mem ps act pc (APut None (Reg (Some r))) = 
+    Some (AS mem (ps(None := ps (Some r))) (Some r) pc)"
+| "assm_step mem ps act pc (APut None (Reg None)) = Some (AS mem ps act pc)"
+| "assm_step mem ps act pc (APut None (Con k)) = Some (AS mem (ps(None := k)) None pc)"
+| "assm_step mem ps act pc (APut (Some r) (Reg (Some r'))) = 
+    Some (AS (mem_upd mem (Some r) (ps (Some r)) (Some r', ps (Some r'))) ps act pc)"
+| "assm_step mem ps act pc (APut (Some r) (Reg None)) = 
+    Some (AS (mem_upd mem (Some r) (ps (Some r)) (act, ps None)) ps act pc)"
+| "assm_step mem ps act pc (APut (Some r) (Con k)) = 
+    Some (AS (mem_upd mem (Some r) (ps (Some r)) (None, k)) ps act pc)"
+| "assm_step mem ps act pc (ASub (Some r) k) = 
+    (if ps (Some r) \<ge> k then Some (AS mem (ps(Some r := ps (Some r) - k)) act pc) else None)"
+| "assm_step mem ps None pc (ASub None k) = None"
+| "assm_step mem ps (Some r) pc (ASub None k) =
+    (if ps None \<ge> k then Some (AS mem (ps(None := ps None - k)) (Some r) pc) else None)"
+| "assm_step mem ps act pc (AAdd (Some r) k) = 
+    Some (AS mem (ps(Some r := ps (Some r) + k)) act pc)"
+| "assm_step mem ps None pc (AAdd None k) = None"
+| "assm_step mem ps (Some r) pc (AAdd None k) = Some (AS mem (ps(None := ps None + k)) (Some r) pc)"
+| "assm_step mem ps None pc AJmp = Some (AS mem (ps(None := 0)) None (ps None))"
+| "assm_step mem ps (Some r) pc AJmp = None"
 
 fun alg_evala :: "assm list \<Rightarrow> assm_state \<rightharpoonup> assm_state" (infix "\<tturnstile>\<^sub>a" 50) where
-  "cd \<tturnstile>\<^sub>a AS mem ps a act pc = (case pc of
+  "cd \<tturnstile>\<^sub>a AS mem ps act pc = (case pc of
       0 \<Rightarrow> None
-    | Suc pc \<Rightarrow> Option.bind (lookup cd pc) (assm_step mem ps a act pc))"
+    | Suc pc \<Rightarrow> Option.bind (lookup cd pc) (assm_step mem ps act pc))"
 
 primrec iter_evala :: "assm list \<Rightarrow> nat \<Rightarrow> assm_state \<rightharpoonup> assm_state" where
   "iter_evala cd 0 \<Sigma> = Some \<Sigma>"
 | "iter_evala cd (Suc x) \<Sigma> = Option.bind (cd \<tturnstile>\<^sub>a \<Sigma>) (iter_evala cd x)"
 
 inductive evala :: "assm list \<Rightarrow> assm_state \<Rightarrow> assm_state \<Rightarrow> bool" (infix "\<tturnstile> _ \<leadsto>\<^sub>a" 50) where
-  eva_movr [simp]: "lookup cd pc = Some (AMov (Reg r)) \<Longrightarrow> 
-    cd \<tturnstile> AS mem ps a act (Suc pc) \<leadsto>\<^sub>a AS mem ps (ps r) (Some r) pc"
-| eva_movp [simp]: "lookup cd pc = Some (AMov (PC _)) \<Longrightarrow> 
-    cd \<tturnstile> AS mem ps a act (Suc pc) \<leadsto>\<^sub>a AS mem ps pc None pc"
-| eva_movk [simp]: "lookup cd pc = Some (AMov (Con k)) \<Longrightarrow> 
-    cd \<tturnstile> AS mem ps a act (Suc pc) \<leadsto>\<^sub>a AS mem ps k None pc"
-| eva_get [simp]: "lookup cd pc = Some (AGet (Some r)) \<Longrightarrow> mem r (ps r) = (t, b) \<Longrightarrow> 
-    cd \<tturnstile> AS mem ps a act (Suc pc) \<leadsto>\<^sub>a AS mem ps b t pc"
-| eva_geta [simp]: "lookup cd pc = Some (AGet None) \<Longrightarrow> mem m a = (t, b) \<Longrightarrow>
-    cd \<tturnstile> AS mem ps a (Some m) (Suc pc) \<leadsto>\<^sub>a AS mem ps b t pc"
-| eva_putr [simp]: "lookup cd pc = Some (APut r (Reg r')) \<Longrightarrow>
-    cd \<tturnstile> AS mem ps a act (Suc pc) \<leadsto>\<^sub>a AS (mem_upd mem r (ps r) (Some r', ps r')) ps a act pc"
-| eva_putk [simp]: "lookup cd pc = Some (APut r (Con k)) \<Longrightarrow>
-    cd \<tturnstile> AS mem ps a act (Suc pc) \<leadsto>\<^sub>a AS (mem_upd mem r (ps r) (None, k)) ps a act pc"
-| eva_putp [simp]: "lookup cd pc = Some (APut r (PC k)) \<Longrightarrow>
-    cd \<tturnstile> AS mem ps a act (Suc pc) \<leadsto>\<^sub>a AS (mem_upd mem r (ps r) (None, k)) ps a act pc"
-| eva_puta [simp]: "lookup cd pc = Some (APut r (PAcc t)) \<Longrightarrow> 
-    cd \<tturnstile> AS mem ps a act (Suc pc) \<leadsto>\<^sub>a AS (mem_upd mem r (ps r) (act, a)) ps a act pc"
-| eva_suba [simp]: "lookup cd pc = Some (ASub None k) \<Longrightarrow> a \<ge> k \<Longrightarrow> 
-    cd \<tturnstile> AS mem ps a (Some r) (Suc pc) \<leadsto>\<^sub>a AS mem ps (a - k) (Some r) pc"
-| eva_sub [simp]: "lookup cd pc = Some (ASub (Some r) k) \<Longrightarrow> ps r \<ge> k \<Longrightarrow>
-    cd \<tturnstile> AS mem ps a act (Suc pc) \<leadsto>\<^sub>a AS mem (ps(r := ps r - k)) a act pc"
+  eva_movr [simp]: "lookup cd pc = Some (APut None (Reg (Some r))) \<Longrightarrow> 
+    cd \<tturnstile> AS mem ps act (Suc pc) \<leadsto>\<^sub>a AS mem (ps(None := ps (Some r))) (Some r) pc"
+| eva_mova [simp]: "lookup cd pc = Some (APut None (Reg None)) \<Longrightarrow> 
+    cd \<tturnstile> AS mem ps act (Suc pc) \<leadsto>\<^sub>a AS mem ps act pc"
+| eva_movk [simp]: "lookup cd pc = Some (APut None (Con k)) \<Longrightarrow> 
+    cd \<tturnstile> AS mem ps act (Suc pc) \<leadsto>\<^sub>a AS mem (ps(None := k)) None pc"
+| eva_get [simp]: "lookup cd pc = Some (AGet (Some r)) \<Longrightarrow> mem (Some r) (ps (Some r)) = (t, b) \<Longrightarrow> 
+    cd \<tturnstile> AS mem ps act (Suc pc) \<leadsto>\<^sub>a AS mem (ps(None := b)) t pc"
+| eva_geta [simp]: "lookup cd pc = Some (AGet None) \<Longrightarrow> mem (Some m) (ps None) = (t, b) \<Longrightarrow>
+    cd \<tturnstile> AS mem ps (Some m) (Suc pc) \<leadsto>\<^sub>a AS mem (ps(None := b)) t pc"
+| eva_putr [simp]: "lookup cd pc = Some (APut (Some r) (Reg (Some r'))) \<Longrightarrow>
+    cd \<tturnstile> AS mem ps act (Suc pc) \<leadsto>\<^sub>a 
+      AS (mem_upd mem (Some r) (ps (Some r)) (Some r', ps (Some r'))) ps act pc"
+| eva_puta [simp]: "lookup cd pc = Some (APut (Some r) (Reg None)) \<Longrightarrow> 
+    cd \<tturnstile> AS mem ps act (Suc pc) \<leadsto>\<^sub>a 
+      AS (mem_upd mem (Some r) (ps (Some r)) (act, ps None)) ps act pc"
+| eva_putk [simp]: "lookup cd pc = Some (APut (Some r) (Con k)) \<Longrightarrow>
+    cd \<tturnstile> AS mem ps act (Suc pc) \<leadsto>\<^sub>a AS (mem_upd mem (Some r) (ps (Some r)) (None, k)) ps act pc"
+| eva_suba [simp]: "lookup cd pc = Some (ASub None k) \<Longrightarrow> ps None \<ge> k \<Longrightarrow> 
+    cd \<tturnstile> AS mem ps (Some r) (Suc pc) \<leadsto>\<^sub>a AS mem (ps(None := ps None - k)) (Some r) pc"
+| eva_sub [simp]: "lookup cd pc = Some (ASub (Some r) k) \<Longrightarrow> ps (Some r) \<ge> k \<Longrightarrow>
+    cd \<tturnstile> AS mem ps act (Suc pc) \<leadsto>\<^sub>a AS mem (ps(Some r := ps (Some r) - k)) act pc"
 | eva_add [simp]: "lookup cd pc = Some (AAdd (Some r) k) \<Longrightarrow> 
-    cd \<tturnstile> AS mem ps a act (Suc pc) \<leadsto>\<^sub>a AS mem (ps(r := ps r + k)) a act pc"
+    cd \<tturnstile> AS mem ps act (Suc pc) \<leadsto>\<^sub>a AS mem (ps(Some r := ps (Some r) + k)) act pc"
 | eva_adda [simp]: "lookup cd pc = Some (AAdd None k) \<Longrightarrow> 
-    cd \<tturnstile> AS mem ps a (Some r) (Suc pc) \<leadsto>\<^sub>a AS mem ps (a + k) (Some r) pc"
+    cd \<tturnstile> AS mem ps (Some r) (Suc pc) \<leadsto>\<^sub>a AS mem (ps(None := ps None + k)) (Some r) pc"
 | eva_jmp [simp]: "lookup cd pc = Some AJmp \<Longrightarrow> 
-    cd \<tturnstile> AS mem ps a None (Suc pc) \<leadsto>\<^sub>a AS mem ps 0 None a"
+    cd \<tturnstile> AS mem ps None (Suc pc) \<leadsto>\<^sub>a AS mem (ps(None := 0)) None (ps None)"
 
-lemma [simp]: "mem_upd (case_register h e vs sh) Hp x y = case_register (h(x := y)) e vs sh"
-  by (rule+) (simp_all split: register.splits)
+lemma [simp]: "mem_upd (registers_case h e vs sh a) (Some Hp) x y = registers_case (h(x := y)) e vs sh a"
+proof (rule, rule)
+  fix m n
+  show "mem_upd (registers_case h e vs sh a) (Some Hp) x y m n =
+    registers_case (h(x := y)) e vs sh a m n"
+      by (induction m) (simp_all split: register.splits)
+qed
 
-lemma [simp]: "mem_upd (case_register h e vs sh) Env x y = case_register h (e(x := y)) vs sh"
-  by (rule+) (simp_all split: register.splits)
+lemma [simp]: "mem_upd (registers_case h e vs sh a) (Some Env) x y = registers_case h (e(x := y)) vs sh a"
+proof (rule, rule)
+  fix m n
+  show "mem_upd (registers_case h e vs sh a) (Some Env) x y m n =
+    registers_case h (e(x := y)) vs sh a m n"
+      by (induction m) (simp_all split: register.splits)
+qed
 
-lemma [simp]: "mem_upd (case_register h e vs sh) Vals x y = case_register h e (vs(x := y)) sh"
-  by (rule+) (simp_all split: register.splits)
+lemma [simp]: "mem_upd (registers_case h e vs sh a) (Some Vals) x y = registers_case h e (vs(x := y)) sh a"
+proof (rule, rule)
+  fix m n
+  show "mem_upd (registers_case h e vs sh a) (Some Vals) x y m n =
+    registers_case h e (vs(x := y)) sh a m n"
+      by (induction m) (simp_all split: register.splits)
+qed
 
-lemma [simp]: "mem_upd (case_register h e vs sh) Stk x y = case_register h e vs (sh(x := y))"
-  by (rule+) (simp_all split: register.splits)
+lemma [simp]: "mem_upd (registers_case h e vs sh a) (Some Stk) x y = registers_case h e vs (sh(x := y)) a"
+proof (rule, rule)
+  fix m n
+  show "mem_upd (registers_case h e vs sh a) (Some Stk) x y m n =
+    registers_case h e vs (sh(x := y)) a m n"
+      by (induction m) (simp_all split: register.splits)
+qed
 
 lemma [simp]: "(case_register hp ep vp sp)(Hp := x) = case_register x ep vp sp"
   by rule (simp split: register.splits)
@@ -121,13 +143,13 @@ proof (induction n arbitrary: \<Sigma>)
   then show ?case by (cases "cd \<tturnstile>\<^sub>a \<Sigma>") simp_all
 qed simp_all
 
-lemma assm_step_equiv: "(Option.bind (lookup cd pc) (assm_step mem ps a act pc) = Some \<Sigma>) \<Longrightarrow>
-  (cd \<tturnstile> AS mem ps a act (Suc pc) \<leadsto>\<^sub>a \<Sigma>)"
+lemma assm_step_equiv: "(Option.bind (lookup cd pc) (assm_step mem ps act pc) = Some \<Sigma>) \<Longrightarrow>
+  (cd \<tturnstile> AS mem ps act (Suc pc) \<leadsto>\<^sub>a \<Sigma>)"
 proof (cases "lookup cd pc")
   case (Some op)
-  moreover assume "Option.bind (lookup cd pc) (assm_step mem ps a act pc) = Some \<Sigma>"
+  moreover assume "Option.bind (lookup cd pc) (assm_step mem ps act pc) = Some \<Sigma>"
   ultimately show ?thesis 
-    by (induction mem ps a act pc op rule: assm_step.induct) (auto split: if_splits prod.splits)
+    by (induction mem ps act pc op rule: assm_step.induct) (auto split: if_splits prod.splits)
 qed simp_all
 
 lemma alg_evala_equiv: "cd \<tturnstile>\<^sub>a \<Sigma> = Some \<Sigma>' = (cd \<tturnstile> \<Sigma> \<leadsto>\<^sub>a \<Sigma>')"
