13MachineCode/Disassemble.thy
@@ -1,5 +1,5 @@
 theory Disassemble
-  imports MachineCode "../12AssemblyCode/AssemblyCode" "../00Utils/Utils" "../00Utils/Iteration"
+  imports MachineCode "../12AssemblyCode/AssemblyCode"
 begin
 
 primrec register_map :: "register \<Rightarrow> reg" where
@@ -14,26 +14,22 @@ primrec register_offset :: "register \<Rightarrow> nat" where
 | "register_offset Vals = 2"
 | "register_offset Stk = 3"
 
-primrec pseudoreg_size :: "pseudoreg \<Rightarrow> nat" where
-  "pseudoreg_size (Reg r) = 4"
-| "pseudoreg_size (PC _) = 1"
+fun pseudoreg_size :: "move_src \<Rightarrow> nat" where
+  "pseudoreg_size (Reg (Some r)) = 4"
+| "pseudoreg_size (Reg None) = 1"
 | "pseudoreg_size (Con k) = 1"
-| "pseudoreg_size (PAcc _) = 1"
 
 fun pseudoreg_map :: "register option \<times> nat \<Rightarrow> nat" where
   "pseudoreg_map (Some r, x) = 4 * x + register_offset r"
 | "pseudoreg_map (None, x) = x"
 
 fun disassemble' :: "assm \<Rightarrow> mach" where
-  "disassemble' (AMov (Reg r)) = MOV R5 (register_map r)"
-| "disassemble' (AMov (PC _)) = MVP R5"
-| "disassemble' (AMov (Con k)) = LDI R5 k"
-| "disassemble' (AMov (PAcc _)) = undefined"
-| "disassemble' (AGet r) = LOD R5 (case r of Some r \<Rightarrow> register_map r | None \<Rightarrow> R5)"
-| "disassemble' (APut r (Reg r')) = STO (register_map r) (register_map r')"
-| "disassemble' (APut r (PC k)) = STI (register_map r) k"
-| "disassemble' (APut r (Con k)) = STI (register_map r) k"
-| "disassemble' (APut r (PAcc _)) = STO (register_map r) R5"
+  "disassemble' (AGet r) = LOD R5 (case r of Some r \<Rightarrow> register_map r | None \<Rightarrow> R5)"
+| "disassemble' (APut (Some r) (Reg r')) = 
+    STO (register_map r) (case r' of Some r' \<Rightarrow> register_map r' | None \<Rightarrow> R5)"
+| "disassemble' (APut (Some r) (Con k)) = STI (register_map r) k"
+| "disassemble' (APut None (Reg r)) = MOV R5 (case r of Some r \<Rightarrow> register_map r | None \<Rightarrow> R5)"
+| "disassemble' (APut None (Con k)) = LDI R5 k"
 | "disassemble' (ASub r k) = SUB (case r of Some r \<Rightarrow> register_map r | None \<Rightarrow> R5) (4 * k)"
 | "disassemble' (AAdd r k) = ADD (case r of Some r \<Rightarrow> register_map r | None \<Rightarrow> R5) (4 * k)"
 | "disassemble' AJmp = JMP R5"
@@ -48,21 +44,21 @@ fun unmap_mem' :: "nat \<Rightarrow> register \<times> nat" where
 | "unmap_mem' (Suc (Suc (Suc 0))) = (Stk, 0)"
 | "unmap_mem' (Suc (Suc (Suc (Suc x)))) = (case unmap_mem' x of (a, b) \<Rightarrow> (a, Suc b))"
 
-definition unmap_mem :: "(register \<Rightarrow> nat \<Rightarrow> register option \<times> nat) \<Rightarrow> nat \<Rightarrow> nat" where
-  "unmap_mem m x = (case unmap_mem' x of (r, p) \<Rightarrow> pseudoreg_map (m r p))"
+definition unmap_mem :: "(register option \<Rightarrow> nat \<Rightarrow> register option \<times> nat) \<Rightarrow> nat \<Rightarrow> nat" where
+  "unmap_mem m x = (case unmap_mem' x of (r, p) \<Rightarrow> pseudoreg_map (m (Some r) p))"
 
-primrec inv_register_map :: "(register \<Rightarrow> nat) \<Rightarrow> nat \<Rightarrow> register option \<Rightarrow> reg \<Rightarrow> nat" where
-  "inv_register_map rs a t R1 = rs Hp * 4"
-| "inv_register_map rs a t R2 = rs Env * 4 + 1"
-| "inv_register_map rs a t R3 = rs Vals * 4 + 2"
-| "inv_register_map rs a t R4 = rs Stk * 4 + 3"
-| "inv_register_map rs a t R5 = pseudoreg_map (t, a)"
+primrec inv_register_map :: "(register option \<Rightarrow> nat) \<Rightarrow> register option \<Rightarrow> reg \<Rightarrow> nat" where
+  "inv_register_map rs t R1 = rs (Some Hp) * 4"
+| "inv_register_map rs t R2 = rs (Some Env) * 4 + 1"
+| "inv_register_map rs t R3 = rs (Some Vals) * 4 + 2"
+| "inv_register_map rs t R4 = rs (Some Stk) * 4 + 3"
+| "inv_register_map rs t R5 = pseudoreg_map (t, rs None)"
 
 primrec disassemble_state :: "assm_state \<Rightarrow> mach_state" where
-  "disassemble_state (AS mem rs a t pc) = MS (inv_register_map rs a t) (unmap_mem mem) pc"
+  "disassemble_state (AS mem rs t pc) = MS (inv_register_map rs t) (unmap_mem mem) pc"
 
 primrec dissassembleable :: "assm_state \<Rightarrow> nat \<Rightarrow> bool" where
-  "dissassembleable (AS mem rs a t pc) lcd = (pc < lcd)"
+  "dissassembleable (AS mem rs t pc) lcd = (pc < lcd)"
 
 lemma [dest]: "R1 = register_map r \<Longrightarrow> r = Hp"
   by (induction r) simp_all
@@ -110,22 +106,22 @@ proof -
 qed
 
 lemma inv_reg_map_reg: "
-  (inv_register_map ps a act)(R5 := inv_register_map ps a act (register_map r)) = 
-    inv_register_map ps (ps r) (Some r)"
+  (inv_register_map ps act)(R5 := inv_register_map ps act (register_map r)) = 
+    inv_register_map (ps(None := ps (Some r))) (Some r)"
 proof
   fix x
-  show "((inv_register_map ps a act)(R5 := inv_register_map ps a act (register_map r))) x = 
-      inv_register_map ps (ps r) (Some r) x"
+  show "((inv_register_map ps act)(R5 := inv_register_map ps act (register_map r))) x = 
+      inv_register_map (ps(None := ps (Some r))) (Some r) x"
   proof (induction x)
     case R5
     thus ?case by (induction r) simp_all
   qed simp_all
 qed
 
-lemma inv_reg_map_none: "(inv_register_map ps a act)(R5 := k) = inv_register_map ps k None"
+lemma inv_reg_map_none: "(inv_register_map ps act)(R5 := k) = inv_register_map (ps(None := k)) None"
 proof
   fix x
-  show "((inv_register_map ps a act)(R5 := k)) x = inv_register_map ps k None x"
+  show "((inv_register_map ps act)(R5 := k)) x = inv_register_map (ps(None := k)) None x"
     by (induction x) simp_all
 qed
 
@@ -147,81 +143,83 @@ proof (induction k)
   thus ?case by (induction m) (simp_all add: numeral_def)
 qed (simp_all add: numeral_def)
 
-lemma [simp]: "inv_register_map (ps(r := k)) a act R5 = inv_register_map ps a act R5"
+lemma [simp]: "inv_register_map (ps(Some r := k)) act R5 = inv_register_map ps act R5"
   by (induction act) simp_all
 
-lemma [simp]: "inv_register_map (ps(r := ps r + k)) a act = 
-  ((inv_register_map ps a act)
-    (register_map r := inv_register_map ps a act (register_map r) + 4 * k))"
+lemma [simp]: "inv_register_map (ps(Some r := ps (Some r) + k)) act = 
+  ((inv_register_map ps act)
+    (register_map r := inv_register_map ps act (register_map r) + 4 * k))"
 proof
   fix x
-  show "inv_register_map (ps(r := ps r + k)) a act x =
-    ((inv_register_map ps a act)
-      (register_map r := inv_register_map ps a act (register_map r) + 4 * k)) x" 
+  show "inv_register_map (ps(Some r := ps (Some r) + k)) act x =
+    ((inv_register_map ps act)
+      (register_map r := inv_register_map ps act (register_map r) + 4 * k)) x" 
     by (induction x) auto
 qed
 
-lemma [simp]: "(inv_register_map ps a (Some r)) (R5 := 4 * a + register_offset r + 4 * k) = 
-  inv_register_map ps (a + k) (Some r)"
+lemma [simp]: "(inv_register_map ps (Some r)) (R5 := 4 * ps None + register_offset r + 4 * k) = 
+  inv_register_map (ps(None := ps None + k)) (Some r)"
 proof
   fix x
-  show "((inv_register_map ps a (Some r)) (R5 := 4 * a + register_offset r + 4 * k)) x =
-    inv_register_map ps (a + k) (Some r) x" by (induction x) simp_all
+  show "((inv_register_map ps (Some r)) (R5 := 4 * ps None + register_offset r + 4 * k)) x =
+    inv_register_map (ps(None := ps None + k)) (Some r) x" by (induction x) simp_all
 qed
 
-lemma [simp]: "ps r \<ge> k \<Longrightarrow>
-  inv_register_map (ps(r := ps r - k)) a act = ((inv_register_map ps a act)
-    (register_map r := inv_register_map ps a act (register_map r) - 4 * k))"
+lemma [simp]: "ps (Some r) \<ge> k \<Longrightarrow>
+  inv_register_map (ps(Some r := ps (Some r) - k)) act = ((inv_register_map ps act)
+    (register_map r := inv_register_map ps act (register_map r) - 4 * k))"
 proof
   fix x
-  assume "ps r \<ge> k"
-  thus "inv_register_map (ps(r := ps r - k)) a act x =
-    ((inv_register_map ps a act) 
-      (register_map r := inv_register_map ps a act (register_map r) - 4 * k)) x" 
+  assume "ps (Some r) \<ge> k"
+  thus "inv_register_map (ps(Some r := ps (Some r) - k)) act x =
+    ((inv_register_map ps act) 
+      (register_map r := inv_register_map ps act (register_map r) - 4 * k)) x" 
     by (induction x) auto
 qed
 
-lemma [simp]: "a \<ge> k \<Longrightarrow> 
-  (inv_register_map ps a (Some r)) (R5 := 4 * a + register_offset r - 4 * k) = 
-    inv_register_map ps (a - k) (Some r)"
+lemma [simp]: "ps None \<ge> k \<Longrightarrow> 
+  (inv_register_map ps (Some r)) (R5 := 4 * ps None + register_offset r - 4 * k) = 
+    inv_register_map (ps(None := ps None - k)) (Some r)"
 proof
   fix x
-  assume "a \<ge> k"
-  thus "((inv_register_map ps a (Some r))
-    (R5 := 4 * a + register_offset r - 4 * k)) x = inv_register_map ps (a - k) (Some r) x" 
+  assume "ps None \<ge> k"
+  thus "((inv_register_map ps (Some r))
+    (R5 := 4 * ps None + register_offset r - 4 * k)) x = 
+      inv_register_map (ps(None := ps None - k)) (Some r) x" 
     by (induction x) simp_all
 qed
 
-lemma [simp]: "unmap_mem mem (inv_register_map ps a (Some r) (register_map r)) = 
-    pseudoreg_map (mem r (ps r))"
+lemma [simp]: "unmap_mem mem (inv_register_map ps (Some r) (register_map r)) = 
+    pseudoreg_map (mem (Some r) (ps (Some r)))"
   by (induction r) (simp_all add: unmap_mem_def split: prod.splits)
 
-lemma [simp]: "mem r (ps r) = (t, b) \<Longrightarrow> 
-  (inv_register_map ps a act)(R5 := unmap_mem mem (inv_register_map ps a act (register_map r))) = 
-    inv_register_map ps b t"
+lemma [simp]: "mem (Some r) (ps (Some r)) = (t, b) \<Longrightarrow> 
+  (inv_register_map ps act)(R5 := unmap_mem mem (inv_register_map ps act (register_map r))) = 
+    inv_register_map (ps(None := b)) t"
 proof
   fix x
-  assume "mem r (ps r) = (t, b)"
-  thus "((inv_register_map ps a act)(R5 := 
-    unmap_mem mem (inv_register_map ps a act (register_map r)))) x = inv_register_map ps b t x"
+  assume "mem (Some r) (ps (Some r)) = (t, b)"
+  thus "((inv_register_map ps act)(R5 := 
+    unmap_mem mem (inv_register_map ps act (register_map r)))) x = 
+      inv_register_map (ps(None := b)) t x"
   proof (induction x)
     case R5
     thus ?case by (induction r) (simp_all add: unmap_mem_def)
   qed simp_all
 qed
 
-lemma unmap_upd_k: "(unmap_mem mem)(inv_register_map ps a act (register_map r) := k) = 
-  unmap_mem (mem_upd mem r (ps r) (None, k))"
+lemma unmap_upd_k: "(unmap_mem mem)(inv_register_map ps act (register_map r) := k) = 
+    unmap_mem (mem_upd mem (Some r) (ps (Some r)) (None, k))"
   by (rule, induction r) (auto simp add: unmap_mem_def split: prod.splits)
 
 lemma [simp]: "((unmap_mem mem)
-  (inv_register_map ps a act (register_map r) := inv_register_map ps a act (register_map r'))) = 
-    unmap_mem (mem_upd mem r (ps r) (Some r', ps r'))"
+  (inv_register_map ps act (register_map r) := inv_register_map ps act (register_map r'))) = 
+    unmap_mem (mem_upd mem (Some r) (ps (Some r)) (Some r', ps (Some r')))"
 proof
   fix x
   show "((unmap_mem mem)
-    (inv_register_map ps a act (register_map r) := inv_register_map ps a act (register_map r'))) x = 
-      unmap_mem (mem_upd mem r (ps r) (Some r', ps r')) x"
+    (inv_register_map ps act (register_map r) := inv_register_map ps act (register_map r'))) x = 
+      unmap_mem (mem_upd mem (Some r) (ps (Some r)) (Some r', ps (Some r'))) x"
   proof (induction r)
     case Hp
     thus ?case by (induction r') (auto simp add: unmap_mem_def split: prod.splits)
@@ -237,27 +235,30 @@ proof
   qed
 qed
 
-lemma [simp]: "((unmap_mem mem)(inv_register_map ps a act (register_map r) := 
-    pseudoreg_map (act, a))) = unmap_mem (mem_upd mem r (ps r) (act, a))"
+lemma [simp]: "((unmap_mem mem)(inv_register_map ps act (register_map r) := 
+    pseudoreg_map (act, a))) = unmap_mem (mem_upd mem (Some r) (ps (Some r)) (act, a))"
 proof
   fix x
-  show "((unmap_mem mem)(inv_register_map ps a act (register_map r) := 
-    pseudoreg_map (act, a))) x = unmap_mem (mem_upd mem r (ps r) (act, a)) x"
+  show "((unmap_mem mem)(inv_register_map ps act (register_map r) := 
+    pseudoreg_map (act, a))) x = unmap_mem (mem_upd mem (Some r) (ps (Some r)) (act, a)) x"
       by (induction r) (auto simp add: unmap_mem_def split: prod.splits)
 qed
 
-lemma [simp]: "mem m a = (t, b) \<Longrightarrow>  
-  ((inv_register_map ps a (Some m))(R5 := unmap_mem mem (4 * a + register_offset m))) = 
-    inv_register_map ps b t"
+lemma [simp]: "mem (Some m) (ps None) = (t, b) \<Longrightarrow>  
+  ((inv_register_map ps (Some m))(R5 := unmap_mem mem (4 * ps None + register_offset m))) = 
+    inv_register_map (ps(None := b)) t"
 proof 
   fix x
-  assume "mem m a = (t, b)"
-  thus "((inv_register_map ps a (Some m))(R5 := unmap_mem mem (4 * a + register_offset m))) 
-    x = inv_register_map ps b t x"
+  assume "mem (Some m) (ps None) = (t, b)"
+  thus "((inv_register_map ps (Some m))(R5 := unmap_mem mem (4 * ps None + register_offset m))) 
+    x = inv_register_map (ps(None := b)) t x"
       by (induction x) (auto simp add: unmap_mem_def)
 qed
 
-lemma [simp]: "lookup cd pc = Some op \<Longrightarrow> disassemble cd ! pc = disassemble' op"
+lemma [simp]: "(inv_register_map ps act)(R5 := pseudoreg_map (act, ps None)) = inv_register_map ps act"
+  by auto
+
+lemma lookup_disassemble [simp]: "lookup cd pc = Some op \<Longrightarrow> disassemble cd ! pc = disassemble' op"
 proof (induction cd)
   case (Cons op cd)
   thus ?case by (induction pc) (simp_all add: disassemble_def)
@@ -266,82 +267,76 @@ qed simp_all
 theorem correctm [simp]: "cd\<^sub>a \<tturnstile> \<Sigma>\<^sub>a \<leadsto>\<^sub>a \<Sigma>\<^sub>a' \<Longrightarrow> 
   disassemble cd\<^sub>a \<tturnstile> disassemble_state \<Sigma>\<^sub>a \<leadsto>\<^sub>m disassemble_state \<Sigma>\<^sub>a'"
 proof (induction cd\<^sub>a \<Sigma>\<^sub>a \<Sigma>\<^sub>a' rule: evala.induct)
-  case (eva_movr cd pc r mem ps a act)
-  hence "disassemble cd \<tturnstile> MS (inv_register_map ps a act) (unmap_mem mem) (Suc pc) \<leadsto>\<^sub>m 
-    MS ((inv_register_map ps a act)(R5 := (inv_register_map ps a act) (register_map r))) 
+  case (eva_movr cd pc r mem ps act)
+  hence "disassemble cd \<tturnstile> MS (inv_register_map ps act) (unmap_mem mem) (Suc pc) \<leadsto>\<^sub>m 
+    MS ((inv_register_map ps act)(R5 := (inv_register_map ps act) (register_map r))) 
       (unmap_mem mem) pc" by simp
   thus ?case by (simp add: inv_reg_map_reg)
 next
-  case (eva_movp cd pc x mem ps a act)
-  hence "disassemble cd \<tturnstile> MS (inv_register_map ps a act) (unmap_mem mem) (Suc pc) \<leadsto>\<^sub>m
-    MS ((inv_register_map ps a act)(R5 := pc)) (unmap_mem mem) pc" by simp
+  case (eva_mova cd pc mem ps act)
+  hence "disassemble cd \<tturnstile> MS (inv_register_map ps act) (unmap_mem mem) (Suc pc) \<leadsto>\<^sub>m 
+    MS ((inv_register_map ps act)(R5 := (inv_register_map ps act) R5)) 
+      (unmap_mem mem) pc" by simp
+  thus ?case by simp
+next
+  case (eva_movk cd pc k mem ps act)
+  hence "disassemble cd \<tturnstile> MS (inv_register_map ps act) (unmap_mem mem) (Suc pc) \<leadsto>\<^sub>m
+    MS ((inv_register_map ps act)(R5 := k)) (unmap_mem mem) pc" by simp
   thus ?case by (simp add: inv_reg_map_none)
 next
-  case (eva_movk cd pc k mem ps a act)
-  hence "disassemble cd \<tturnstile> MS (inv_register_map ps a act) (unmap_mem mem) (Suc pc) \<leadsto>\<^sub>m
-    MS ((inv_register_map ps a act)(R5 := k)) (unmap_mem mem) pc" by simp
-  thus ?case by (simp add: inv_reg_map_none)
-next
-  case (eva_geta cd pc mem m a t b ps) 
+  case (eva_geta cd pc mem r ps t b) 
   hence "disassemble cd ! pc = LOD R5 R5" by simp
-  hence "disassemble cd \<tturnstile> MS (inv_register_map ps a (Some m)) (unmap_mem mem) (Suc pc) \<leadsto>\<^sub>m 
-    MS ((inv_register_map ps a (Some m))(R5 := unmap_mem mem (inv_register_map ps a (Some m) R5))) 
+  hence "disassemble cd \<tturnstile> MS (inv_register_map ps (Some r)) (unmap_mem mem) (Suc pc) \<leadsto>\<^sub>m 
+    MS ((inv_register_map ps (Some r))(R5 := unmap_mem mem (inv_register_map ps (Some r) R5))) 
       (unmap_mem mem) pc" by (metis evm_lod)
   with eva_geta(2) show ?case by simp
 next
-  case (eva_get cd pc r mem ps t b a act)
+  case (eva_get cd pc r mem ps t b act)
   hence "disassemble cd ! pc = LOD R5 (register_map r)" by simp
-  hence "disassemble cd \<tturnstile> MS (inv_register_map ps a act) (unmap_mem mem) (Suc pc) \<leadsto>\<^sub>m
-    MS ((inv_register_map ps a act)(R5 := (unmap_mem mem) ((inv_register_map ps a act) 
+  hence "disassemble cd \<tturnstile> MS (inv_register_map ps act) (unmap_mem mem) (Suc pc) \<leadsto>\<^sub>m
+    MS ((inv_register_map ps act)(R5 := (unmap_mem mem) ((inv_register_map ps act) 
       (register_map r)))) (unmap_mem mem) pc" by (metis evm_lod)
   with eva_get(2) show ?case by simp
 next
-  case (eva_puta cd pc r act mem ps a t)
+  case (eva_puta cd pc r mem ps act)
   hence "disassemble cd ! pc = STO (register_map r) R5" by simp
-  hence "disassemble cd \<tturnstile> MS (inv_register_map ps a t) (unmap_mem mem) (Suc pc) \<leadsto>\<^sub>m
-    MS (inv_register_map ps a t) ((unmap_mem mem)(inv_register_map ps a t (register_map r) := 
-      inv_register_map ps a t R5)) pc" by (metis evm_sto)
+  hence "disassemble cd \<tturnstile> MS (inv_register_map ps act) (unmap_mem mem) (Suc pc) \<leadsto>\<^sub>m
+    MS (inv_register_map ps act) ((unmap_mem mem)(inv_register_map ps act (register_map r) := 
+      inv_register_map ps act R5)) pc" by (metis evm_sto)
   thus ?case by simp
 next
-  case (eva_putp cd pc r k mem ps a act)
-  hence "disassemble cd ! pc = STI (register_map r) k" by simp
-  hence "disassemble cd \<tturnstile> MS (inv_register_map ps a act) (unmap_mem mem) (Suc pc) \<leadsto>\<^sub>m 
-    MS (inv_register_map ps a act) ((unmap_mem mem)((inv_register_map ps a act) (register_map r) := 
-      k)) pc" by (metis evm_sti)
-  thus ?case by (simp add: unmap_upd_k)
-next
-  case (eva_putr cd pc r r' mem ps a act)
+  case (eva_putr cd pc r r' mem ps act)
   hence "disassemble cd ! pc = STO (register_map r) (register_map r')" by simp
-  hence "disassemble cd \<tturnstile> MS (inv_register_map ps a act) (unmap_mem mem) (Suc pc) \<leadsto>\<^sub>m
-    MS (inv_register_map ps a act) ((unmap_mem mem)(inv_register_map ps a act (register_map r) := 
-      inv_register_map ps a act (register_map r'))) pc" by (metis evm_sto)
+  hence "disassemble cd \<tturnstile> MS (inv_register_map ps act) (unmap_mem mem) (Suc pc) \<leadsto>\<^sub>m
+    MS (inv_register_map ps act) ((unmap_mem mem)(inv_register_map ps act (register_map r) := 
+      inv_register_map ps act (register_map r'))) pc" by (metis evm_sto)
   thus ?case by simp
 next
-  case (eva_putk cd pc r k mem ps a act)
+  case (eva_putk cd pc r k mem ps act)
   hence "disassemble cd ! pc = STI (register_map r) k" by simp
-  hence "disassemble cd \<tturnstile> MS (inv_register_map ps a act) (unmap_mem mem) (Suc pc) \<leadsto>\<^sub>m
-    MS (inv_register_map ps a act) 
-      ((unmap_mem mem)(inv_register_map ps a act (register_map r) := k)) pc" by (metis evm_sti)
+  hence "disassemble cd \<tturnstile> MS (inv_register_map ps act) (unmap_mem mem) (Suc pc) \<leadsto>\<^sub>m
+    MS (inv_register_map ps act) 
+      ((unmap_mem mem)(inv_register_map ps act (register_map r) := k)) pc" by (metis evm_sti)
   thus ?case by (simp add: unmap_upd_k)
 next
-  case (eva_suba cd pc k a mem ps r)
+  case (eva_suba cd pc k ps mem r)
   hence "disassemble cd ! pc = SUB R5 (4 * k)" by simp
-  hence "disassemble cd \<tturnstile> MS (inv_register_map ps a (Some r)) (unmap_mem mem) (Suc pc) \<leadsto>\<^sub>m 
-    MS ((inv_register_map ps a (Some r))(R5 := inv_register_map ps a (Some r) R5 - 4 * k)) 
+  hence "disassemble cd \<tturnstile> MS (inv_register_map ps (Some r)) (unmap_mem mem) (Suc pc) \<leadsto>\<^sub>m 
+    MS ((inv_register_map ps (Some r))(R5 := inv_register_map ps (Some r) R5 - 4 * k)) 
       (unmap_mem mem) pc" by (metis evm_sub)
   with eva_suba show ?case by simp
 next
-  case (eva_adda cd pc k mem ps a r)
+  case (eva_adda cd pc k mem ps r)
   hence "disassemble cd ! pc = ADD R5 (4 * k)" by simp
-  hence "disassemble cd \<tturnstile> MS (inv_register_map ps a (Some r)) (unmap_mem mem) (Suc pc) \<leadsto>\<^sub>m 
-    MS ((inv_register_map ps a (Some r))(R5 := inv_register_map ps a (Some r) R5 + 4 * k)) 
+  hence "disassemble cd \<tturnstile> MS (inv_register_map ps (Some r)) (unmap_mem mem) (Suc pc) \<leadsto>\<^sub>m 
+    MS ((inv_register_map ps (Some r))(R5 := inv_register_map ps (Some r) R5 + 4 * k)) 
       (unmap_mem mem) pc" by (metis evm_add)
   with eva_adda show ?case by simp
 next
-  case (eva_jmp cd pc mem ps a)
+  case (eva_jmp cd pc mem ps)
   hence "disassemble cd ! pc = JMP R5" by simp
-  hence "disassemble cd \<tturnstile> MS (inv_register_map ps a None) (unmap_mem mem) (Suc pc) \<leadsto>\<^sub>m 
-    MS ((inv_register_map ps a None)(R5 := 0)) (unmap_mem mem) (inv_register_map ps a None R5)" 
+  hence "disassemble cd \<tturnstile> MS (inv_register_map ps None) (unmap_mem mem) (Suc pc) \<leadsto>\<^sub>m 
+    MS ((inv_register_map ps None)(R5 := 0)) (unmap_mem mem) (inv_register_map ps None R5)" 
       by (metis evm_jmp)
   thus ?case by (simp add: inv_reg_map_none)
 qed simp_all
@@ -349,19 +344,19 @@ qed simp_all
 theorem correctm_iter [simp]: "iter (\<tturnstile> cd\<^sub>a \<leadsto>\<^sub>a) \<Sigma>\<^sub>a \<Sigma>\<^sub>a' \<Longrightarrow> 
     iter (\<tturnstile> disassemble cd\<^sub>a \<leadsto>\<^sub>m) (disassemble_state \<Sigma>\<^sub>a) (disassemble_state \<Sigma>\<^sub>a')"
   by (induction \<Sigma>\<^sub>a \<Sigma>\<^sub>a' rule: iter.induct) (simp, metis correctm iter_append iter_one)
- 
-lemma [simp]: "inv_register_map (case_register 0 0 0 2) 0 None = case_reg 0 1 2 11 0" 
+
+lemma [simp]: "inv_register_map (registers_case 0 0 0 2 0) None = case_reg 0 1 2 11 0" 
   by (auto split: reg.splits)
 
-lemma [simp]: "inv_register_map (case_register hp ep (Suc 0) 0) 0 None = 
+lemma [simp]: "inv_register_map (registers_case hp ep (Suc 0) 0 0) None = 
     case_reg (4 * hp) (Suc (4 * ep)) 6 3 0"
   by (auto split: reg.splits)
 
 lemma [dest]: "unmap_mem' x = (r, y) \<Longrightarrow> x = 4 * y + register_offset r"
   by (induction x arbitrary: y rule: unmap_mem'.induct) (simp_all split: prod.splits)
 
-lemma [simp]: "unmap_mem (case_register (\<lambda>x. (None, 0)) (\<lambda>x. (None, 0)) (\<lambda>x. (None, 0)) 
-  ((\<lambda>x. (None, 0))(0 := (None, 0), Suc 0 := (Some Env, 0)))) = (\<lambda>x. 0)(7 := 1)"
+lemma [simp]: "unmap_mem (registers_case (\<lambda>x. (None, 0)) (\<lambda>x. (None, 0)) (\<lambda>x. (None, 0)) 
+  ((\<lambda>x. (None, 0)) (0 := (None, 0), Suc 0 := (Some Env, 0))) undefined) = (\<lambda>x. 0)(7 := 1)"
 proof (rule, unfold unmap_mem_def)
   fix x
   obtain r p where R: "unmap_mem' x = (r, p)" by fastforce
@@ -371,8 +366,8 @@ proof (rule, unfold unmap_mem_def)
       | _ \<Rightarrow> (\<lambda>x. (None, 0))) p) = ((\<lambda>x. 0)(3 := 0, 7 := 1)) x" 
     by (induction r) (simp_all, presburger+)
   with R show "(case unmap_mem' x of (r, p) \<Rightarrow> 
-    pseudoreg_map ((case r of 
-      Stk \<Rightarrow> (\<lambda>x. (None, 0))(0 := (None, 0), Suc 0 := (Some Env, 0)) | _ \<Rightarrow> (\<lambda>x. (None, 0))) p)) =
+    pseudoreg_map (registers_case (\<lambda>x. (None, 0)) (\<lambda>x. (None, 0)) (\<lambda>x. (None, 0))
+      ((\<lambda>x. (None, 0))(0 := (None, 0), Suc 0 := (Some Env, 0))) undefined (Some r) p)) =
         ((\<lambda>x. 0)(7 := 1)) x" by simp
 qed
 
